Factor WfReflective through WfReflectiveGen

src/Reflection/WfReflective.v
@@ -49,6 +49,7 @@
 
 Require Import Coq.Arith.Arith Coq.Logic.Eqdep_dec.
 Require Import Crypto.Reflection.Syntax.
+Require Import Crypto.Reflection.WfReflectiveGen.
 Require Import Crypto.Util.Notations Crypto.Util.Tactics Crypto.Util.Option Crypto.Util.Sigma Crypto.Util.Prod Crypto.Util.Decidable Crypto.Util.ListUtil.
 Require Export Crypto.Util.PointedProp. (* export for the [bool >-> option pointed_Prop] coercion *)
 Require Export Crypto.Util.FixCoqMistakes.
@@ -88,263 +89,19 @@ Section language.
   Local Notation interp_flat_type := (interp_flat_type_gen interp_base_type).
   Local Notation exprf := (@exprf base_type_code interp_base_type op).
   Local Notation expr := (@expr base_type_code interp_base_type op).
+  Local Notation duplicate_type := (@duplicate_type base_type_code var1 var2).
+  Local Notation reflect_wffT := (@reflect_wffT base_type_code interp_base_type interp_base_type base_type_eq_semidec_transparent op (fun _ => eq) op_beq var1 var2).
+  Local Notation reflect_wfT := (@reflect_wfT base_type_code interp_base_type interp_base_type base_type_eq_semidec_transparent op (fun _ => eq) op_beq var1 var2).
+  Local Notation flat_type_eq_semidec_transparent := (@flat_type_eq_semidec_transparent base_type_code base_type_eq_semidec_transparent).
+  Local Notation preflatten_binding_list2 := (@preflatten_binding_list2 base_type_code base_type_eq_semidec_transparent var1 var2).
+  Local Notation type_eq_semidec_transparent := (@type_eq_semidec_transparent base_type_code base_type_eq_semidec_transparent).
 
-  Local Ltac inversion_base_type_code_step :=
-    match goal with
-    | [ H : ?x = ?x :> base_type_code |- _ ]
-      => assert (H = eq_refl) by eapply UIP_dec, dec_rel_of_semidec_rel, base_type_eq_semidec_is_dec; subst H
-    | [ H : ?x = ?y :> base_type_code |- _ ] => subst x || subst y
-    end.
-  Local Ltac inversion_base_type_code := repeat inversion_base_type_code_step.
-
-  (* lift [base_type_eq_semidec_transparent] across [flat_type] *)
-  Fixpoint flat_type_eq_semidec_transparent (t1 t2 : flat_type) : option (t1 = t2)
-    := match t1, t2 return option (t1 = t2) with
-       | Syntax.Tbase t1, Syntax.Tbase t2
-         => option_map (@f_equal _ _ Tbase _ _)
-                      (base_type_eq_semidec_transparent t1 t2)
-       | Syntax.Tbase _, _ => None
-       | Prod A B, Prod A' B'
-         => match flat_type_eq_semidec_transparent A A', flat_type_eq_semidec_transparent B B' with
-           | Some p, Some q => Some (f_equal2 Prod p q)
-           | _, _ => None
-           end
-       | Prod _ _, _ => None
-       end.
-  Fixpoint type_eq_semidec_transparent (t1 t2 : type) : option (t1 = t2)
-    := match t1, t2 return option (t1 = t2) with
-       | Syntax.Tflat t1, Syntax.Tflat t2
-         => option_map (@f_equal _ _ (@Tflat _) _ _)
-                      (flat_type_eq_semidec_transparent t1 t2)
-       | Syntax.Tflat _, _ => None
-       | Arrow A B, Arrow A' B'
-         => match base_type_eq_semidec_transparent A A', type_eq_semidec_transparent B B' with
-           | Some p, Some q => Some (f_equal2 (@Arrow base_type_code) p q)
-           | _, _ => None
-           end
-       | Arrow _ _, _ => None
-       end.
-  Lemma base_type_eq_semidec_transparent_refl t : base_type_eq_semidec_transparent t t = Some eq_refl.
+  Lemma interp_flat_type_gen_rel_pointwise2_eq {t} (x y : interp_flat_type t)
+    : interp_flat_type_gen_rel_pointwise2 (fun _ => eq) x y <-> x = y.
   Proof.
-    clear -base_type_eq_semidec_is_dec.
-    pose proof (base_type_eq_semidec_is_dec t t).
-    destruct (base_type_eq_semidec_transparent t t); intros; try intuition congruence.
-    inversion_base_type_code; reflexivity.
+    induction t; simpl in *; [ reflexivity | ].
+    rewrite_hyp !*; intuition (simpl in *; try congruence).
   Qed.
-  Lemma flat_type_eq_semidec_transparent_refl t : flat_type_eq_semidec_transparent t t = Some eq_refl.
-  Proof.
-    clear -base_type_eq_semidec_is_dec.
-    induction t as [t | A B IHt]; simpl.
-    { rewrite base_type_eq_semidec_transparent_refl; reflexivity. }
-    { rewrite_hyp !*; reflexivity. }
-  Qed.
-  Lemma type_eq_semidec_transparent_refl t : type_eq_semidec_transparent t t = Some eq_refl.
-  Proof.
-    clear -base_type_eq_semidec_is_dec.
-    induction t as [t | A B IHt]; simpl.
-    { rewrite flat_type_eq_semidec_transparent_refl; reflexivity. }
-    { rewrite base_type_eq_semidec_transparent_refl; rewrite_hyp !*; reflexivity. }
-  Qed.
-
-  Definition op_beq' t1 tR t1' tR' (x : op t1 tR) (y : op t1' tR') : option pointed_Prop
-    := match flat_type_eq_semidec_transparent t1 t1', flat_type_eq_semidec_transparent tR tR' with
-       | Some p, Some q
-         => match p in (_ = t1'), q in (_ = tR') return op t1' tR' -> _ with
-           | eq_refl, eq_refl => fun y => op_beq _ _ x y
-           end y
-       | _, _ => None
-       end.
-
-  (** While [Syntax.wff] is parameterized over a list of [sigT (fun t
-      => var1 t * var2 t)], it is simpler here to make everything
-      heterogenous, rather than trying to mix homogenous and
-      heterogenous things.† Thus we parameterize our [reflect_wffT]
-      over a list of [sigT (fun t => var1 (fst t) * var2 (snd t))],
-      and write a function ([duplicate_type]) that turns the former
-      into the latter.
-
-      † This is an instance of the general theme that abstraction
-        barriers are important.  Here we enforce the abstraction
-        barrier that our input decision procedures are homogenous, but
-        all of our internal code is strictly heterogenous.  This
-        allows us to contain the conversions between homogenous and
-        heterogenous code to a few functions: [op_beq'],
-        [eq_type_and_var], [eq_type_and_const], and to the statement
-        about [Syntax.wff] itself.  *)
-
-  Definition eq_semidec_and_gen {T} (semidec : forall x y : T, option (x = y))
-             (t t' : T) (f : T -> Type) (x : f t) (x' : f t')
-    : option pointed_Prop
-    := match semidec t t' with
-       | Some p
-         => Some (inject (eq_rect _ f x _ p = x'))
-       | None => None
-       end.
-
-  (* Here is where we use the generality of [pointed_Prop], to say
-     that two things of type [var1] are equal, and two things of type
-     [var2] are equal. *)
-  Definition eq_type_and_var : sigT eP -> sigT eP -> option pointed_Prop
-    := fun x y => (eq_semidec_and_gen
-                  base_type_eq_semidec_transparent _ _ var1 (fst (projT2 x)) (fst (projT2 y))
-                /\ eq_semidec_and_gen
-                    base_type_eq_semidec_transparent _ _ var2 (snd (projT2 x)) (snd (projT2 y)))%option_pointed_prop.
-  Definition eq_type_and_const (t t' : flat_type) (x : interp_flat_type t) (y : interp_flat_type t')
-    : option pointed_Prop
-    := eq_semidec_and_gen
-         flat_type_eq_semidec_transparent _ _ interp_flat_type x y.
-
-  Definition duplicate_type (ls : list (sigT (fun t => var1 t * var2 t)%type)) : list (sigT eP)
-    := List.map (fun v => existT eP (projT1 v, projT1 v) (projT2 v)) ls.
-
-  Lemma duplicate_type_app ls ls'
-    : (duplicate_type (ls ++ ls') = duplicate_type ls ++ duplicate_type ls')%list.
-  Proof. apply List.map_app. Qed.
-  Lemma duplicate_type_length ls
-    : List.length (duplicate_type ls) = List.length ls.
-  Proof. apply List.map_length. Qed.
-  Lemma duplicate_type_in t v ls
-    : List.In (existT _ (t, t) v) (duplicate_type ls) -> List.In (existT _ t v) ls.
-  Proof.
-    unfold duplicate_type; rewrite List.in_map_iff.
-    intros [ [? ?] [? ?] ].
-    inversion_sigma; inversion_prod; inversion_base_type_code; subst; simpl.
-    assumption.
-  Qed.
-  Lemma duplicate_type_not_in G t t0 v (H : base_type_eq_semidec_transparent t t0 = None)
-    : ~List.In (existT _ (t, t0) v) (duplicate_type G).
-  Proof.
-    apply base_type_eq_semidec_is_dec in H.
-    clear -H; intro H'.
-    induction G as [|? ? IHG]; simpl in *; destruct H';
-      intuition; congruence.
-  Qed.
-
-  Definition preflatten_binding_list2 t1 t2 : option (forall (x : interp_flat_type_gen var1 t1) (y : interp_flat_type_gen var2 t2), list (sigT (fun t => var1 t * var2 t)%type))
-    := match flat_type_eq_semidec_transparent t1 t2 with
-       | Some p
-         => Some (fun x y
-                 => let x := eq_rect _ (interp_flat_type_gen var1) x _ p in
-                   flatten_binding_list base_type_code x y)
-       | None => None
-       end.
-  Definition flatten_binding_list2 t1 t2 : option (forall (x : interp_flat_type_gen var1 t1) (y : interp_flat_type_gen var2 t2), list (sigT eP))
-    := option_map (fun f x y => duplicate_type (f x y)) (preflatten_binding_list2 t1 t2).
-  (** This function adds De Bruijn indices to variables *)
-  Fixpoint natize_interp_flat_type_gen var t (base : nat) (v : interp_flat_type_gen var t) {struct t}
-    : nat * interp_flat_type_gen (fun t : base_type_code => nat * var t)%type t
-    := match t return interp_flat_type_gen var t -> nat * interp_flat_type_gen _ t with
-       | Prod A B => fun v => let ret := @natize_interp_flat_type_gen _ A base (fst v) in
-                          let base := fst ret in
-                          let a := snd ret in
-                          let ret := @natize_interp_flat_type_gen _ B base (snd v) in
-                          let base := fst ret in
-                          let b := snd ret in
-                          (base, (a, b))
-       | Syntax.Tbase t => fun v => (S base, (base, v))
-       end v.
-  Arguments natize_interp_flat_type_gen {var t} _ _.
-  Lemma length_natize_interp_flat_type_gen1 {t} (base : nat) (v1 : interp_flat_type_gen var1 t) (v2 : interp_flat_type_gen var2 t)
-    : fst (natize_interp_flat_type_gen base v1) = length (flatten_binding_list base_type_code v1 v2) + base.
-  Proof.
-    revert base; induction t; simpl; [ reflexivity | ].
-    intros; rewrite List.app_length, <- plus_assoc.
-    rewrite_hyp <- ?*; reflexivity.
-  Qed.
-  Lemma length_natize_interp_flat_type_gen2 {t} (base : nat) (v1 : interp_flat_type_gen var1 t) (v2 : interp_flat_type_gen var2 t)
-    : fst (natize_interp_flat_type_gen base v2) = length (flatten_binding_list base_type_code v1 v2) + base.
-  Proof.
-    revert base; induction t; simpl; [ reflexivity | ].
-    intros; rewrite List.app_length, <- plus_assoc.
-    rewrite_hyp <- ?*; reflexivity.
-  Qed.
-
-  (* This function strips De Bruijn indices from expressions *)
-  Fixpoint unnatize_exprf {var t} (base : nat) (e : @exprf (fun t => nat * var t)%type t) : @exprf var t
-    := match e in @Syntax.exprf _ _ _ _ t return exprf t with
-       | Const _ x => Const x
-       | Var _ x => Var (snd x)
-       | Op _ _ op args => Op op (@unnatize_exprf _ _ base args)
-       | LetIn _ ex _ eC => LetIn (@unnatize_exprf _ _ base ex)
-                             (fun x => let v := natize_interp_flat_type_gen base x in
-                                    @unnatize_exprf _ _ (fst v) (eC (snd v)))
-       | Pair _ x _ y => Pair (@unnatize_exprf _ _ base x) (@unnatize_exprf _ _ base y)
-       end.
-  Fixpoint unnatize_expr {var t} (base : nat) (e : @expr (fun t => nat * var t)%type t) : @expr var t
-    := match e in @Syntax.expr _ _ _ _ t return expr t with
-       | Return _ x => unnatize_exprf base x
-       | Abs tx tR f => Abs (fun x : var tx => let v := natize_interp_flat_type_gen (t:=tx) base x in
-                                           @unnatize_expr _ _ (fst v) (f (snd v)))
-       end.
-
-  Fixpoint reflect_wffT (G : list (sigT (fun t => var1 (fst t) * var2 (snd t))%type))
-           {t1 t2 : flat_type}
-           (e1 : @exprf (fun t => nat * var1 t)%type t1) (e2 : @exprf (fun t => nat * var2 t)%type t2)
-           {struct e1}
-    : option pointed_Prop
-    := match e1, e2 return option _ with
-       | Const t0 x, Const t1 y
-         => match flat_type_eq_semidec_transparent t0 t1 with
-           | Some p => Some (inject (eq_rect _ interp_flat_type x _ p = y))
-           | None => None
-           end
-       | Const _ _, _ => None
-       | Var t0 x, Var t1 y
-         => match beq_nat (fst x) (fst y), List.nth_error G (List.length G - S (fst x)) with
-           | true, Some v => eq_type_and_var v (existT _ (t0, t1) (snd x, snd y))
-           | _, _ => None
-           end
-       | Var _ _, _ => None
-       | Op t1 tR op args, Op t1' tR' op' args'
-         => match @reflect_wffT G t1 t1' args args', op_beq' t1 tR t1' tR' op op' with
-           | Some p, Some q => Some (p /\ q)%pointed_prop
-           | _, _ => None
-           end
-       | Op _ _ _ _, _ => None
-       | LetIn tx ex tC eC, LetIn tx' ex' tC' eC'
-         => match @reflect_wffT G tx tx' ex ex', @flatten_binding_list2 tx tx', flat_type_eq_semidec_transparent tC tC' with
-           | Some p, Some G0, Some _
-             => Some (p /\ inject (forall (x : interp_flat_type_gen var1 tx) (x' : interp_flat_type_gen var2 tx'),
-                                    match @reflect_wffT (G0 x x' ++ G)%list _ _
-                                                       (eC (snd (natize_interp_flat_type_gen (List.length G) x)))
-                                                       (eC' (snd (natize_interp_flat_type_gen (List.length G) x'))) with
-                                    | Some p => to_prop p
-                                    | None => False
-                                    end))
-           | _, _, _ => None
-           end
-       | LetIn _ _ _ _, _ => None
-       | Pair tx ex ty ey, Pair tx' ex' ty' ey'
-         => match @reflect_wffT G tx tx' ex ex', @reflect_wffT G ty ty' ey ey' with
-           | Some p, Some q => Some (p /\ q)
-           | _, _ => None
-           end
-       | Pair _ _ _ _, _ => None
-       end%pointed_prop.
-
-    Fixpoint reflect_wfT (G : list (sigT (fun t => var1 (fst t) * var2 (snd t))%type))
-           {t1 t2 : type}
-           (e1 : @expr (fun t => nat * var1 t)%type t1) (e2 : @expr (fun t => nat * var2 t)%type t2)
-           {struct e1}
-    : option pointed_Prop
-    := match e1, e2 return option _ with
-       | Return _ x, Return _ y
-         => reflect_wffT G x y
-       | Return _ _, _ => None
-       | Abs tx tR f, Abs tx' tR' f'
-         => match @flatten_binding_list2 tx tx', type_eq_semidec_transparent tR tR' with
-           | Some G0, Some _
-             => Some (inject (forall (x : interp_flat_type_gen var1 tx) (x' : interp_flat_type_gen var2 tx'),
-                                match @reflect_wfT (G0 x x' ++ G)%list _ _
-                                                   (f (snd (natize_interp_flat_type_gen (List.length G) x)))
-                                                   (f' (snd (natize_interp_flat_type_gen (List.length G) x'))) with
-                                | Some p => to_prop p
-                                | None => False
-                                end))
-           | _, _ => None
-           end
-       | Abs _ _ _, _ => None
-       end%pointed_prop.
 
   Local Ltac handle_op_beq_correct :=
     repeat match goal with
@@ -357,6 +114,8 @@ Section language.
     | _ => progress unfold eq_type_and_var, op_beq', flatten_binding_list2, preflatten_binding_list2, option_map, and_option_pointed_Prop, eq_semidec_and_gen in *
     | _ => progress simpl in *
     | _ => progress break_match
+    | [ H : interp_flat_type_gen_rel_pointwise2 (fun _ => eq) _ _ |- _ ]
+      => apply interp_flat_type_gen_rel_pointwise2_eq in H
     | _ => progress subst
     | _ => progress inversion_option
     | _ => progress inversion_pointed_Prop
@@ -384,7 +143,7 @@ Section language.
       => erewrite length_natize_interp_flat_type_gen1, length_natize_interp_flat_type_gen2; eassumption
     | [ H : base_type_eq_semidec_transparent _ _ = None |- False ] => eapply duplicate_type_not_in; eassumption
     | [ H : List.nth_error _ _ = Some _ |- _ ] => apply List.nth_error_In in H
-    | [ H : List.In _ (duplicate_type _) |- _ ] => apply duplicate_type_in in H
+    | [ H : List.In _ (duplicate_type _) |- _ ] => eapply duplicate_type_in in H; [ | eassumption.. ]
     | [ H : context[match _ with _ => _ end] |- _ ] => revert H; progress break_match
     | [ |- wff _ _ _ ] => constructor
     | [ |- wf _ _ _ ] => constructor
@@ -468,8 +227,8 @@ Section Wf.
   (** Leads to smaller proofs, but is less generally applicable *)
   Theorem reflect_Wf_unnatize
     : (forall var1 var2,
-          prop_of_option (@reflect_wfT base_type_code interp_base_type base_type_eq_semidec_transparent op op_beq var1 var2 nil t t (e _) (e _)))
-      -> Wf (fun var => unnatize_expr base_type_code interp_base_type op 0 (e (fun t => (nat * var t)%type))).
+          prop_of_option (@reflect_wfT base_type_code interp_base_type interp_base_type base_type_eq_semidec_transparent op (fun _ => eq) op_beq var1 var2 nil t t (e _) (e _)))
+      -> Wf (fun var => unnatize_expr 0 (e (fun t => (nat * var t)%type))).
   Proof.
     intros H var1 var2; specialize (H var1 var2).
     pose proof (@reflect_wf base_type_code interp_base_type base_type_eq_semidec_transparent base_type_eq_semidec_is_dec op op_beq op_beq_bl var1 var2 nil t t (e _) (e _)) as H'.
@@ -481,8 +240,8 @@ Section Wf.
       size of the expression tree), but more generally applicable *)
   Theorem reflect_Wf
     : (forall var1 var2,
-          unnatize_expr base_type_code interp_base_type op 0 (e (fun t => (nat * var1 t)%type)) = e _
-          /\ prop_of_option (@reflect_wfT base_type_code interp_base_type base_type_eq_semidec_transparent op op_beq var1 var2 nil t t (e _) (e _)))
+          unnatize_expr 0 (e (fun t => (nat * var1 t)%type)) = e _
+          /\ prop_of_option (@reflect_wfT base_type_code interp_base_type interp_base_type base_type_eq_semidec_transparent op (fun _ => eq) op_beq var1 var2 nil t t (e _) (e _)))
       -> Wf e.
   Proof.
     intros H var1 var2.
